Foundation/Modal/Neighborhood/Supplementation.lean
@@ -8,19 +8,19 @@ namespace LO.Modal.Neighborhood
 
 variable {F : Frame}
 
-def Frame.Supplementation (F : Frame) : Frame := Frame.mk_ℬ F.World (λ X => (Set.sUnion { F.box Y | Y ⊆ X }))
+def Frame.supplementation (F : Frame) : Frame := Frame.mk_ℬ F.World (λ X => (Set.sUnion { F.box Y | Y ⊆ X }))
 
-namespace Frame.Supplementation
+namespace Frame.supplementation
 
-lemma iff_exists_subset {X : Set (F.World)} {w : F.World} : w ∈ F.Supplementation.box X ↔ ∃ Y ⊆ X, w ∈ F.box Y := by
-  simp [Frame.Supplementation, Frame.box, Frame.mk_ℬ, Set.mem_sUnion, Set.mem_setOf_eq, exists_exists_and_eq_and]
+lemma iff_exists_subset {X : Set (F.World)} {w : F.World} : w ∈ F.supplementation.box X ↔ ∃ Y ⊆ X, w ∈ F.box Y := by
+  simp [Frame.supplementation, Frame.box, Frame.mk_ℬ, Set.mem_sUnion, Set.mem_setOf_eq, exists_exists_and_eq_and]
 
-lemma subset (X : Set (F.World)) : F.box X ⊆ F.Supplementation.box X := by
+lemma subset (X : Set (F.World)) : F.box X ⊆ F.supplementation.box X := by
   intro x;
-  simp [Frame.Supplementation, Frame.box, Frame.mk_ℬ];
+  simp [Frame.supplementation, Frame.box, Frame.mk_ℬ];
   tauto;
 
-lemma monotonic {X Y : Set (F.World)} (h : X ⊆ Y) : F.Supplementation.box X ⊆ F.Supplementation.box Y := by
+lemma monotonic {X Y : Set (F.World)} (h : X ⊆ Y) : F.supplementation.box X ⊆ F.supplementation.box Y := by
   intro x hX;
   obtain ⟨X', hX', hX⟩ := iff_exists_subset.mp hX;
   apply iff_exists_subset.mpr;
@@ -29,7 +29,7 @@ lemma monotonic {X Y : Set (F.World)} (h : X ⊆ Y) : F.Supplementation.box X �
   . apply Set.Subset.trans hX' h;
   . assumption;
 
-lemma monotonic_iterated {X Y : Set (F.World)} (h : X ⊆ Y) (n) : F.Supplementation.box^[n] X ⊆ F.Supplementation.box^[n] Y := by
+lemma monotonic_iterated {X Y : Set (F.World)} (h : X ⊆ Y) (n) : F.supplementation.box^[n] X ⊆ F.supplementation.box^[n] Y := by
   induction n with
   | zero => simpa;
   | succ n ih =>
@@ -37,9 +37,9 @@ lemma monotonic_iterated {X Y : Set (F.World)} (h : X ⊆ Y) (n) : F.Supplementa
     apply monotonic;
     apply ih;
 
-lemma itl_reduce : F.Supplementation.Supplementation.box X = F.Supplementation.box X := by
+lemma itl_reduce : F.supplementation.supplementation.box X = F.supplementation.box X := by
   ext x;
-  simp only [Supplementation, mk_ℬ, Set.mem_setOf_eq, Set.mem_sUnion, exists_exists_and_eq_and]
+  simp only [supplementation, mk_ℬ, Set.mem_setOf_eq, Set.mem_sUnion, exists_exists_and_eq_and]
   constructor;
   . rintro ⟨Y, RYX, Z, RZY, hZ⟩;
     use Z;
@@ -48,7 +48,7 @@ lemma itl_reduce : F.Supplementation.Supplementation.box X = F.Supplementation.b
     . assumption;
   . tauto;
 
-instance isMonotonic : F.Supplementation.IsMonotonic := by
+instance isMonotonic : F.supplementation.IsMonotonic := by
   constructor;
   rintro X Y x hx;
   obtain ⟨W, hW₁, hW₂⟩ := iff_exists_subset.mp hx;
@@ -59,7 +59,7 @@ instance isMonotonic : F.Supplementation.IsMonotonic := by
     . tauto_set;
     . assumption;
 
-instance isReflexive [F.IsReflexive] : F.Supplementation.IsReflexive := by
+instance isReflexive [F.IsReflexive] : F.supplementation.IsReflexive := by
   constructor;
   intro X w hw;
   replace ⟨Y, hY₁, hY₂⟩ := iff_exists_subset.mp hw;
@@ -67,14 +67,14 @@ instance isReflexive [F.IsReflexive] : F.Supplementation.IsReflexive := by
   apply F.refl;
   exact hY₂;
 
-instance [F.ContainsUnit] : F.Supplementation.ContainsUnit := by
+instance [F.ContainsUnit] : F.supplementation.ContainsUnit := by
   constructor;
   ext x;
-  suffices ∃ a, a ∈ F.𝒩 x by simpa [Supplementation, mk_ℬ];
+  suffices ∃ a, a ∈ F.𝒩 x by simpa [supplementation, mk_ℬ];
   use Set.univ;
   simp;
 
-instance isTransitive [F.IsTransitive] : F.Supplementation.IsTransitive := by
+instance isTransitive [F.IsTransitive] : F.supplementation.IsTransitive := by
   constructor;
   intro X w hw;
   obtain ⟨Y, hYX, hY⟩ := iff_exists_subset.mp hw;
@@ -82,7 +82,7 @@ instance isTransitive [F.IsTransitive] : F.Supplementation.IsTransitive := by
   apply monotonic $ subset Y;
   apply subset (F.box Y) $ F.trans hY;
 
-instance isRegular [F.IsRegular] : F.Supplementation.IsRegular := by
+instance isRegular [F.IsRegular] : F.supplementation.IsRegular := by
   constructor;
   rintro X Y w ⟨hX, hY⟩;
   apply iff_exists_subset.mpr;
@@ -94,7 +94,7 @@ instance isRegular [F.IsRegular] : F.Supplementation.IsRegular := by
   . apply @Frame.regular F _ X' Y';
     tauto;
 
-end Frame.Supplementation
+end Frame.supplementation
 
 
 section
@@ -108,7 +108,7 @@ open MaximalConsistentSet.proofset
 variable {S} [Entailment (Formula ℕ) S]
 variable {𝓢 : S} [Entailment.EM 𝓢] [Entailment.Consistent 𝓢]
 
-abbrev maximalCanonicalFrame (𝓢 : S) [Entailment.E 𝓢] [Entailment.Consistent 𝓢] : Frame := (minimalCanonicalFrame 𝓢).Supplementation
+abbrev maximalCanonicalFrame (𝓢 : S) [Entailment.E 𝓢] [Entailment.Consistent 𝓢] : Frame := (minimalCanonicalFrame 𝓢).supplementation
 
 namespace maximalCanonicalFrame
 
@@ -116,7 +116,7 @@ open Classical in
 lemma box_proofset : Frame.box (maximalCanonicalFrame 𝓢) (proofset 𝓢 φ) = proofset 𝓢 (□φ) := by
   ext Γ;
   suffices (∃ a ⊆ proofset 𝓢 φ, Γ ∈ if h : ∃ φ, a = proofset 𝓢 φ then proofset 𝓢 (□h.choose) else ∅) ↔ Γ ∈ proofset 𝓢 (□φ) by
-    simpa [maximalCanonicalFrame, minimalCanonicalFrame, Frame.mk_ℬ, Frame.Supplementation];
+    simpa [maximalCanonicalFrame, minimalCanonicalFrame, Frame.mk_ℬ, Frame.supplementation];
   constructor;
   . rintro ⟨X, hX₁, hX₂⟩;
     split_ifs at hX₂ with hX;
